nits

examples/wysteria/sem.fst
@@ -965,25 +965,43 @@ val compose_vals: #m1:v_meta -> #m2:v_meta -> v1:value m1 -> v2:value m2
                  -> Tot (r:dvalue{compose_v_meta_inv m1 m2 (D_v.meta r)})
                     (decreases %[v1])
 val compose_envs: en:env -> env -> Tot (varname -> Tot (option dvalue)) (decreases %[en])
-
 let rec compose_vals #m1 #m2 v1 v2 =
  if is_v_emp v1 then D_v m2 v2
  else if is_v_emp v2 then D_v m1 v1
  else
    let emp = D_v (Meta empty Can_b empty Can_w) V_emp in
    match v1 with
-     | V_prin _
-     | V_eprins _
-     | V_prins _
-     | V_unit
-     | V_bool _ -> D_v m1 v1
+     | V_prin p1 ->
+       if is_v_prin v2 && V_prin.c v1 = V_prin.c v2 then
+	 D_v m1 v1
+       else emp
+       
+     | V_eprins eps1 ->
+       if is_v_eprins v2 && V_eprins.c v1 = V_eprins.c v2 then
+	 D_v m1 v1
+       else emp
+
+     | V_prins ps1 ->
+       if is_v_prins v2 && V_prins.c v1 = V_prins.c v2 then
+	 D_v m1 v1
+       else emp
+
+     | V_unit ->
+       if is_v_unit v2 then
+	 D_v m1 v1
+       else emp
+
+     | V_bool b1 ->
+       if is_v_bool v2 && V_bool.c v1 = V_bool.c v2 then
+	 D_v m1 v1
+       else emp
 
      | V_opaque 'a v1 m1 s1 c1 sps1 ->
        if is_v_opaque v2 then
 	 let V_opaque 'b v2 m2 s2 c2 sps2 = v2 in
 	 let c1' = Mk_c_w c1 in
 	 let c2' = Mk_c_w c2 in
-	 if verified_eq c1' c2' then
+	 if c1' = c2' then
 	   let v' = c1 v1 v2 in
 	   let m' = compose_opaque_meta m1 m2 in
 	   D_v m' (V_opaque v' m' s1 c1 sps1)
@@ -996,7 +1014,8 @@ let rec compose_vals #m1 #m2 v1 v2 =
          if ps1 = ps2 then
            let D_v meta v = compose_vals v1 v2 in
            D_v (Meta ps1 Can_b (Meta.wps meta) Cannot_w) (V_box ps1 v)
-         else emp
+         else
+           emp
        else emp
 
      | V_wire eps1 w1 ->
@@ -1011,25 +1030,25 @@ let rec compose_vals #m1 #m2 v1 v2 =
      | V_clos en1 x1 e1 ->
        if is_v_clos v2 then
          let V_clos en2 x2 e2 = v2 in
-         (*if x1 = x2 && e1 = e2 then*)
+         if x1 = x2 && e1 = e2 then
            D_v m1 (V_clos (compose_envs en1 en2) x1 e1)
-         (*else emp*)
+         else emp
        else emp
 
      | V_fix_clos en1 f1 x1 e1 ->
        if is_v_fix_clos v2 then
          let V_fix_clos en2 f2 x2 e2 = v2 in
-         (*if f1 = f2 && x1 = x2 && e1 = e2 then*)
+         if f1 = f2 && x1 = x2 && e1 = e2 then
            D_v m1 (V_fix_clos (compose_envs en1 en2) f1 x1 e1)
-         (*else emp*)
+         else emp
        else emp
 
      | V_emp_clos x1 e1 ->
        if is_v_emp_clos v2 then
          let V_emp_clos x2 e2 = v2 in
-         (*if x1 = x2 && e1 = e2 then*)
+         if x1 = x2 && e1 = e2 then
            D_v m1 (V_emp_clos x1 e1)
-         (*else emp*)
+         else emp
        else emp
 
 and compose_envs en1 en2 =
